**Textbook sections**: 3.4, 3.5

# Complex Eigenvalues (3.4)

For a real matrix with complex eigenvalues, we are given a complex conjugate pair of eigenvalues. 

Select one of these eigenvalues & its corresponding eigenvector:
$$
\lambda = \alpha + i\beta\quad\vec v = \vec a + i\vec b
$$

The general solution is
$$
\begin{align*}
\vec x_1 &= e^{\alpha t}(\vec a \cos (\beta t) - \vec b\sin (\beta t) )\\
\vec x_2 &= e^{\alpha t}(\vec a\sin (\beta t) + \vec b \cos (\beta t))\\
\vec x &= c_1 \vec x_1 + c_2 \vec x_2.
\end{align*}
$$

> [!Info]+ Derivation
> Note that a solution to the system is
> $$\vec u = e^{\lambda t}\vec v.$$
> 
> Using our definitions above, we can expand:
> $$
\begin{align*}
\vec u &= e^{\lambda t}\vec v\\
&= e^{\alpha t}e^{i \beta t}(\vec a + i \vec b)\\
&= e^{\alpha t}(\cos (\beta t) + i\sin(\beta t))(\vec a + i \vec b)\\
&= e^{\alpha t}((\vec a\cos (\beta t) - \vec b \sin (\beta t)) + i(\vec a \sin (\beta t) + \vec b \cos (\beta t)))\\
&= \overbrace{e^{\alpha t}(\vec a \cos (\beta t) - \vec b\sin (\beta t) )}^{\vec x_1} + i\overbrace{ e^{\alpha t}(\vec a\sin (\beta t) + \vec b \cos (\beta t))}^{\vec x_2}\\
&= \vec x_1 + i\vec x_2
\end{align*}
> $$
>
> Hence, the general solution is
> $$
\begin{align*}
\vec x_1 &= e^{\alpha t}(\vec a \cos (\beta t) - \vec b\sin (\beta t) )\\
\vec x_2 &= e^{\alpha t}(\vec a\sin (\beta t) + \vec b \cos (\beta t))\\
\vec x &= c_1 \vec x_1 + c_2 \vec x_2
\end{align*}
> $$
> 
> *Note that the conjugate eigenvalue and eigenvector will result in the same $\vec x_1$ and $\vec x_2$.*

See: [[03d. Phase Portraits#Complex Eigenvalues|phase portraits]].

> [!Example]+
> Determine general solution to
> $$
\vec x' = \begin{bmatrix}-1 & 2 \\ -1 & -3\end{bmatrix}\vec x
> $$
> 
> ### Computing eigenthings
> Eigenvectors:
> $$
\begin{align*}
(-1-\lambda)(-3-\lambda)+2 &= 0\\
\lambda^2 +4\lambda+5&=0\\
\lambda&=-2\pm \sqrt{4 - 5}\\
&= -2 \pm i
\end{align*}
> $$
> Eigenvalues:
> $$(A - \lambda I)\vec v = \begin{bmatrix}-1-\lambda & 2 \\ -1 & -3 - \lambda\end{bmatrix} \vec v = 0$$
> $\lambda_1 = - 2 - i$:
> $$A - \lambda I = \begin{bmatrix}1 + i & 2 \\ -1 & -1 + i\end{bmatrix}$$
> $$\vec v_1 = \begin{bmatrix}-1 + i \\ 1\end{bmatrix}$$
> $\lambda_2 = - 2 + i$:
> $$A - \lambda I = \begin{bmatrix}1 - i & 2 \\ -1 & -1 - i\end{bmatrix}$$
> $$\vec v_2 = \begin{bmatrix}-1 - i \\ 1\end{bmatrix}$$
> 
> ### General solution
> 
> Using $\lambda_2 = -2 + i$:
> $$\begin{align*}
\alpha &= -2,\\
\beta &= 1\\
\vec a &= \begin{bmatrix}-1 \\ 1\end{bmatrix}\\
\vec b &= \begin{bmatrix}-1 \\ 0\end{bmatrix}
\end{align*}
> $$
>
> So the general solution:
> $$
\begin{align*}
\vec x_1 &= e^{-2t}\left(\begin{bmatrix}-1 \\ 1\end{bmatrix}\cos t - \begin{bmatrix}-1 \\ 0\end{bmatrix} \sin t\right)\\
\vec x_2 &= e^{-2t}\left(\begin{bmatrix}-1 \\ 1\end{bmatrix}\sin t + \begin{bmatrix}-1 \\ 0\end{bmatrix} \cos t\right)\\
\vec x &= c_1 \vec x_1 + c_2 \vec x_2
\end{align*}
> $$

# Repeated Eigenvalues (3.5)

In a situation where there's a repeated eigenvalue but not two eigenvectors, the solution found will be:
$$
\vec r(t) = c_1 e^{\lambda t} \vec v + c_2 e^{\lambda t}(\vec vt + \vec w)
$$

$\vec w$ can be found by finding independent solutions to $(A - \lambda I)\vec w = \vec v$ (this is known as a **generalized eigenvector**).

See: [[03d. Phase Portraits#Repeated Eigenvalues|phase portraits]].

> [!Info]+ Motivating Example 1
> Given an object moving in the plane with motion $\vec{r}(t) = \begin{bmatrix}x(t) \\ y(t)\end{bmatrix}$, such that the velocity is defined as:
> $$
\begin{align*}
x' &= -x + ky\\
y' &= -y
\end{align*}
> $$
> and such that $\vec{r}(0) = \begin{bmatrix}1 \\ 2\end{bmatrix}$.
> 
> ### $k = 0$
> $$
\begin{align*}
\frac{d\vec r}{dt} = \begin{bmatrix}-1 & 0 \\ 0 & -1\end{bmatrix}\vec r
\end{align*}
> $$
> 
> We can compute the eigenvalues as
> $$(-1 - \lambda)^2 = 0$$
> So $\lambda_1 = \lambda_2 = -1$.
> 
> The eigenvectors are: $\begin{bmatrix}1 \\ 0\end{bmatrix}, \begin{bmatrix}0 \\ 1\end{bmatrix}.$
> 
> #### Phase Portrait
> ![[03c-1-repeated-ex1-pp.png]]
> 
> ### $k \neq 0$
> 
> There aren't two eigenvectors so we can't use the matrix method.
> 
> Since $y' = -y$, we know that $y = c_2e^{-t}$.
> 
> We can then substitute and solve for $x' + x = ky$:
> $$
\begin{align*}
e^{t}x' + e^tx &= e^t ky\\
e^t x &= \int kc_2\,dt\\
x &= \frac{kc_2t}{e^t} + \frac{c_1}{e^t}
\end{align*}
> $$
> 
> Hence:
> $$
\begin{align*}
\vec{r} &= \begin{bmatrix}c_1e^{-t} + kc_2te^{-t} \\ c_2e^{-t} \end{bmatrix}\\
&= c_1e^{-t}\begin{bmatrix}1 \\ 0\end{bmatrix} + c_2e^{-t}\left(\begin{bmatrix}1 \\ 0\end{bmatrix}kt + \begin{bmatrix}0 \\ 1\end{bmatrix}\right)
\end{align*}
> $$
> #### Phase Portrait
>
> ![[03c-2-repeated-ex2-pp.png]]

> [!Info]+ Motivating Example 2
> Find the general solution to the given system:
> $$\vec x' = \begin{bmatrix}1 & -1 \\ 1 & 3\end{bmatrix}\vec{x}.$$
> 
> ## First Solution
> In computing the eigenvalues and eigenvectors, we find $\lambda_1 = \lambda_2 = 2$, and $\vec v = \begin{bmatrix}1 \\ -1\end{bmatrix}$.
> 
> Hence, one of our solutions is $\vec x_1 = e^{2t}\begin{bmatrix}1 \\ -1\end{bmatrix}$.
> 
> ## Second Solution
> 
> Is there another linearly independent solution?
> 
> Motivating Example 1 indicates that our 2nd solution is of the form $e^{2t}(t\vec v + \vec w)$. As such, assume $$\vec x_2 = e^{2t}(t\vec v + \vec w).$$
> Note that:
> $$
\begin{align*}
\vec x_2' &= \frac{d}{dt}(te^{2t}\vec v + e^{2t}\vec w)\\
&= e^{2t}\vec v + 2te^{2t}\vec v + 2e^{2t}\vec{w},
\end{align*}
> $$
> and:
> $$
\begin{align*}
\vec{x}_2' &= A\vec{x}_2\\
&= A(te^{2t}\vec v + e^{2t}\vec w).
\end{align*}
> $$
> 
> Setting these equal, we have
> $$
\begin{align*}
e^{2t}\vec v + 2te^{2t}\vec v + 2e^{2t}\vec{w} &= A(te^{2t}\vec v + e^{2t}\vec w)\\
\vec v + 2t\vec v + 2\vec{w} &= A(t\vec v) + A\vec w
\end{align*}
> $$
> 
> Aligning the $t$ and non-$t$ terms:
> $$
\begin{align*}
A(t\vec{v}) &= 2t\vec v\\
\vec v + 2\vec w &= A\vec w
\end{align*}
> $$
> We are trying to find $(A - 2I)\vec w = \vec v$, so solve:
> $$
\begin{bmatrix}
-1 & -1 \\ 1 & 1
\end{bmatrix} \vec w = \begin{bmatrix}-1 \\1\end{bmatrix}
> $$
> 
> In solving this, we find $w_1 + w_2 = 1$, leaving the solution $\vec w = \begin{bmatrix}w_1 \\ 1 - w_1\end{bmatrix} = \begin{bmatrix}0 \\ 1\end{bmatrix} + w_1\begin{bmatrix}1 \\ -1\end{bmatrix}.$
> 
> Thus, our second solution is $\vec x_2 = e^{2t}\left(t\begin{bmatrix}1 \\ -1\end{bmatrix} + \begin{bmatrix}0 \\ 1\end{bmatrix}\right).$
> 
> *(Note: the extra $w_1\begin{bmatrix}1 \\ -1\end{bmatrix}$ from our derivation of $\vec w$ would join with $\vec x_1$.)*
