**Textbook sections**: 4.5, 4.7
There are two methods of finding a particular solution.

# Method of Undetermined Coefficients (4.5)

## Examples
1. $y'' + 3y' + 2y = 10e^{3t}$

Testing $y = Ae^{3t}$, we get
$$
\begin{align*}
9Ae^{3t} + 9Ae^{3t} + 2e^{3t} &= 10e^{3t}\\
20Ae^{3t} &= 10e^{3t}\\
a &= \frac{1}{2}
\end{align*}
$$
2. $y'' + 3y' + 2y = \sin t$

Testing $y = A \cos t + B \sin t$,
$$
\begin{align*}
(-A \cos t - B \sin t) + 3(-A \sin t + B \cos t) + 2(A \cos t + B \sin t) &= \sin t\\
(-3A + B) \sin t + (A + 3B)\cos t &= \sin t
\end{align*}
$$
We can solve, getting $A = - \frac{3}{10}, B = \frac{1}{10}$

3. $y'' - 6y' + 9y = e^{3t}$

Testing $y = Ae^{3t}$, we get
$$
\begin{align*}
9Ae^{3t} - 18Ae^{3t} + 9Ae^{3t} &= e^{3t}\\
0 &= e^{3t}
\end{align*}
$$
$e^{3t}$ is a solution to the homo problem, so cannot be used.

Testing $y = Ate^{3t}$,
solution fails for the same reason.

Testing $y = At^2 e^{3t}$.

$$
\begin{align*}
y' &= 2Ate^{3t} + 3At^2 e^3t\\
y'' &= 2Ae^{3t} + 12Ate^{3t} + 9At^2 e^{3t}
\end{align*}
$$
Do some math.
This does work and can be used to solve it.

## Strategy for Undetermined Coefficients

To solve $$ay'' + by' + cy = g(t),$$
1. Obtain the general solution of the homo sol'n.
2. Determine if undetermined coefficients can be used.*
3. If RHS is a sum, do the problem for the individual terms.
	4. Find a particular solution for each problem. Assume particular solution form, determine coefficients.
	5. Repeat for all terms.
6. Form general solution & solve IVP

\*Undetermined coefficients can only be used for polynomials, sin/cos, exponentials.
Let: 
- $P_n$ be some polynomials of degree $n$ 
- $Q_n, R_n$ be polynomials of deg $n$ (with undetermined coefficients)

|$g(t)$|particular solution $Y(t)$|
|-|-|
|$P_n$|$t^{*} \times Q_n$|
| $P_n e^{\alpha t}$|$t^* \times e^{\alpha t} \times Q_n$|
| $P_n e^{\alpha t} \sin(\beta t)$, $P_n e^{\alpha t} \cos(\beta t)$|$t^* \times e^{\alpha t}(\cos(\beta t)Q_n + \sin(\beta t) R_n)$|
$t^*$ designates the smallest exponent of $t$ such that the particular solution is not a solution in the homogeneous counterpart.

# Variation of Parameters (4.7)
Limitations of undetermined coefficients:
- Does not give an explicit expression for the particular solution
- Can only be applied for sine, cosine, exponentials, and polynomials

## Strategy for Variation of Parameters

We seek a solution to nonhomogeneous:
$$
y'' + p(t)y' + q(t)y = g(t).
$$
(Note $y''$ coefficient is 1.)

The solution to corresponding homo problem is:
$$
y_h = c_1 y_1(t) + c_2 y_2(t)
$$
To find a particular solution, replace $c_1, c_2$ with functions $v_1, v_2$, and try to find those functions.
$$
y_p = v_1(t)y_1(t) + v_2(t)y_2(t)
$$

### Procedure for Variation of Parameters (for SOLDEs)

1. Solve homogeneous problem to find $y_1, y_2$.
2. Solve the system of nonlinear equations:
$$
\begin{align*}
y_1 v_1' + y_2 v_2' &= 0\\
y_1' v_1' + y_2' v_2' &= g
\end{align*}
$$
3. Integrate $v_1', v_2'$ to get $v_1, v_2$.
4. $y_p = v_1 y_1  + v_2 y_2$.

(Alternatively, $$y_p = -y_1 \int \frac{y_2 g}{W[y_1, y_2]}\,dt+y_2\int\frac{y_1g}{W[y_1, y_2]}\,dt$$)

#### Derivation
$$y_p = v_1 y_1  + v_2 y_2.$$
Then,
$$y_p' = v_1 y_1' + v_2 y_2' + v_1' y_1 + v_2' y_2.$$
For simplicity's sake, let $v_1' y_1 + v_2' y_2 = 0$.

Then,
$$
\begin{align*}
y_p' &= v_1 y_1' + v_2 y_2'\\
y_p'' &= v_1' y_1' + v_2' y_2' + v_1 y_1'' + v_2y_2''
\end{align*}
$$
Substituting:
$$
\begin{align*}
y_p'' + py_p' + qy_p &= (v_1' y_1' + v_2' y_2' + v_1 y_1'' + v_2y_2'') + p(v_1 y_1' + v_2 y_2') + q(v_1 y_1  + v_2 y_2)\\
&= v_1(y_1'' + py_1' + qy_1) + v_2(y_2'' + py_2' + qy_2) + v_1'(y_1') + v_2'(y_2')\\
&= v_1'y_1' + v_2'y_2'
\end{align*}
$$

As such, we get our two constraints:
$$
\begin{align*}
y_1 v_1' + y_2 v_2' &= 0\\
y_1' v_1' + y_2' v_2' &= g
\end{align*}
$$

#### Example
Determine a particular solution to
$$
t^2 y'' - 4ty' + 6y = 4t^3, \quad t>0
$$
given that $y_1 = t^2, y_2 = t^3$ are solutions to the homogeneous equation.

Standard form:
$$
y'' - \frac{4}{t}y' + \frac{6}{t^2}y = 4t.
$$
$$
\begin{align*}
t^2 v_1' + t^3 v_2' &= 0\\
2t v_1' + 3t^2 v_2' &= 4t
\end{align*}
$$
Note that $(2) \times t$:
$$
\begin{align*}
2t^2v_1' + 3t^3v_2' &= 4t^2\\
t^3v_2' &= 4t^2\\
v_2' &= \frac{4}{t}
\end{align*}
$$
Then, substituting into (1):

$$
\begin{align*}
t^2 v_1' + 4t^2 &= 0\\
t^2 v_1'&= -4t^2\\
v_1'&= -4
\end{align*}
$$

Integrating, we get:
$$
\begin{align*}
v_1 &= -4t\\
v_2 &= 4\ln t
\end{align*}
$$
So our particular solution is:
$$
y_p = -4t^3 +  4 t^3 \ln t
$$

### Strategy for Variation of Parameters (for Systems of FOLDEs)
We seek a solution to nonhomogeneous:
$$
\begin{align*}
\vec x_1' = P\vec x + \vec g(t)
\end{align*}
$$
($P$ being some matrix function, $\vec g$ being some vector function)

If the solution to the corresponding homogeneous problem is
$$
\vec x_h = c_1 \vec x_1(t) + c_2 \vec x_2(t),
$$
a particular solution can be obtained by replacing $c_1, c_2$ with scalar functions $v_1, v_2$:
$$
\vec x_p = v_1(t) \vec x_1(t) + v_2(t) \vec x_2(t)
$$

We define the **fundamental matrix**: $$X(t) = \begin{bmatrix}\vec x_1 & \vec x_2\end{bmatrix}$$
There is a particular solution:
$$
\vec x_p = X(t) \int \overbrace{X^{-1}(t) \vec g(t)}^{\text{solution to } [X \mid \vec g]}\,dt
$$
#### Derivation

Assume
$$
\begin{align*}
\vec x_p &= v_1(t) \vec x_1(t) + v_2(t) \vec x_2(t)\\
&= \begin{bmatrix}\vec x_1 & \vec x_2\end{bmatrix}\begin{bmatrix}v_1 \\ v_2\end{bmatrix}\\
&= X\vec v.
\end{align*}
$$
Note that:
$$\vec x_p' = X' \vec v + X \vec v'.$$


Substituting into the equation:
$$
\begin{align*}
\vec x_p' &= P\vec x_p + \vec g\\
X' \vec v + X \vec v' &= P(X \vec v) + \vec g
\end{align*}
$$
Note that $PX = X'$.
$$
\begin{align*}
X' \vec v + X \vec v' &= X'\vec v + \vec g\\
X\vec v'&= \vec g
\end{align*}
$$

#### Example
Determine a particular solution to
$$
\vec x_1 = \begin{bmatrix}2 & -3 \\ 1 & -2\end{bmatrix}\vec x(t) + \begin{bmatrix}e^{2t} \\ 1\end{bmatrix}
$$
given the solutions to the homogeneous equation are
$$
\begin{align*}
\vec x_1 &= e^t\begin{bmatrix}3 \\ 1\end{bmatrix}\\
\vec x_2 &= e^{-t}\begin{bmatrix}1 \\ 1\end{bmatrix}
\end{align*}
$$

The fundamental matrix:
$$
X = \begin{bmatrix}3e^t & e^{-t} \\ e^t & e^{-t}\end{bmatrix}
$$
Then, solving $[X | \vec g]$:
$$
\begin{align*}
\begin{bmatrix}3e^t & e^{-t} & \bigm| & e^{2t}\\ e^t & e^{-t} & \bigm| & 1\end{bmatrix}\\
\begin{bmatrix}3e^{2t} & 1 & \bigm| & e^{3t}\\ 3e^{2t} & 3 & \bigm| & 3e^t\end{bmatrix}\\
\begin{bmatrix}3e^{2t} & 1 & \bigm| & e^{3t}\\ 0 & 2 & \bigm| & 3e^t - e^{3t}\end{bmatrix}\\
\begin{bmatrix}3e^{2t} & 1 & \bigm| & \frac{3e^{3t}}{2}\\ 0 & 1 & \bigm| & \frac{3e^t}{2} - \frac{e^{3t}}{2}\end{bmatrix}\\
\begin{bmatrix}3e^{2t} & 0 & \bigm| & \frac{3e^{3t}}{2} - \frac{3e^t}{2}\\ 0 & 1 & \bigm| & \frac{3e^t}{2} - \frac{e^{3t}}{2}\end{bmatrix}\\
\begin{bmatrix}1 & 0 & \bigm| & \frac{e^{t}}{2} - \frac{e^{-t}}{2}\\ 0 & 1 & \bigm| & \frac{3e^t}{2} - \frac{e^{3t}}{2}\end{bmatrix}
\end{align*}
$$
Then,
$$
\begin{align*}
\vec x_p &= X(t) \int X^{-1}(t) \vec g(t)\,dt\\
&=\frac{1}{2}X\int\begin{bmatrix}e^t - e^{-t} \\ 3e^t - e^{3t} \end{bmatrix}\,dt\\
&= \frac{1}{2}\begin{bmatrix}3e^t & e^{-t} \\ e^t & e^{-t}\end{bmatrix}\begin{bmatrix}e^t + e^{-t} \\ 3e^t - \frac{1}{3}e^{3t}\end{bmatrix}\\
&= \frac{1}{2}\begin{bmatrix}(3e^{2t} + 3) + (3 - \frac{1}{3}e^{2t}) \\ (e^{2t} + 1) + (3 - \frac{1}{3}e^{2t})\end{bmatrix}\\
&= \frac{1}{2}\begin{bmatrix}\frac{8}{3}e^{2t} + 6 \\ \frac{2}{3}e^{2t} + 4\end{bmatrix}\\
&= \begin{bmatrix}\frac{4}{3}e^{2t} + 3 \\ \frac{1}{3}e^{2t} + 2\end{bmatrix}
\end{align*}
$$