**Textbook sections**: 5.1, 5.2, 5.3, 5.4

> [!Info]+ Motivating Example
> 
> ![[12-1-motivating-example.png]]
> 
> Let the mass of salt (n ikg) in the tank at time $t$ be $x(t)$. The tank holds 1000 L, and $x(0) = 0$.
> 
> The concentration of salt flowing into the tank is given by:
> $$g(t) = \begin{cases}
>  0.04\text{ kg/L} \cdot 6\text{ L/min}, & 0 < t < 10\\
>  0.02\text{ kg/L} \cdot 6\text{ L/min}, & 10 < t
> \end{cases}$$
> 
> ### Solving
> 
> You could:
>  - Solve at $t \in (0, 10)$ to obtain $x(10)$,
>  - Use that to solve situation at $t \in (10, \infty)$.
>  
>  However, as the piecewise gets increasingly complicated, this becomes unmaintainable.

The Laplace transform is useful as it lets us redefine our equations to something that may be easier to solve for (and a process that may be easier to solve for), and then transform back.

# Definition of Laplace Transform (5.1)

Suppose $f(t)$ is defined on $[0, \infty)$. Then, the **Laplace Transform** is
$$
\mathcal L\{f\}(s) = \int_0^\infty e^{-st}f(t)\,dt.
$$
The domain of $\mathcal L\{f\}$ is the set of values where the integral exists.

> [!Example]+ Example: $\mathcal L\{1\}$ 
> $$
> \begin{align*}
>   \mathcal L\{1\}(s) &= \int_0^\infty e^{-st}\,dt\\
>   &= \left.-\frac{1}{s}e^{-st}\right|^{t=\infty}_{t=0}\\
>   &= - \frac{1}{s}(0 - 1)\\
>   &= \frac{1}{s}
> \end{align*}
> $$

> [!Example]+ Example: $\mathcal L\{e^{at}\}$ 
> $$
> \begin{align*}
>   \mathcal L\{1\}(s) &= \int_0^\infty e^{-st}e^{at}\,dt\\
>   &= \int_0^\infty e^{(a-s)t}\,dt\\
>   &= \left.\frac{1}{a - s}e^{(a -s)t}\right|^{t=\infty}_{t=0}\\
>   &= \frac{1}{a - s}(0 - 1), \quad s > a\\
>   &= \frac{1}{s - a}, \quad s > a
> \end{align*}
> $$

> [!Example]+ Example: $\mathcal L\{\sin at\}$
> $$
> \begin{align*}
>   \sin at &= \frac{1}{2i}(e^{iat} - e^{-iat})\\
>   \mathcal L\{\sin at\} &= \frac{1}{2i}\left(\frac{1}{s-ia} - \frac{1}{s+ia}\right)\\
>   &= \frac{a}{s^2 + a^2}
> \end{align*}
> $$

> [!Example]+ $\mathcal L$ for a piecewise continuous function
> Let 
> $$
> f(t) = \begin{cases}
>   e^2t, & 0 \leq t < 1\\
>   4, & 1 \leq t
> \end{cases}
> $$
> 
> Compute $\mathcal L\{f\}$.
> $$
> \begin{align*}
>   \mathcal L\{f\} &= \int_0^\infty fe^{-st}\,dt\\
>   &= \int_0^1 e^{2t}e^{-st}\,dt + \int_1^\infty 4e^{-st}\,dt\\
>   &= \left.\left(\frac{1}{2-s}e^{(2-s)t}\right)\right|^{t=1}_{t=0} - \left.\left(\frac{4}{s}e^{-st}\right)\right|^{t=\infty}_{t=1}\\
>   &= \frac{e^{2 - s} - 1}{2-s} + \frac{4e^{-s}}{s}\quad s>0, s\ne 2
> \end{align*}
> $$

## Linearity

The Laplace transform is a **linear operator**:
$$
\begin{align*}
\mathcal L\{f + g\} &= \mathcal L\{f\} + \mathcal L\{g\}\\
\mathcal L\{kf\} &= k\mathcal L\{f\}
\end{align*}
$$

## Exponential Order

What conditions must be satisfied for the Laplace transform of $f$ to exist?

$f$ is of **exponential order** if there exists constants $K, a, M$ such that
$$|f(t)| \leq Ke^{at},$$
for all $t > M$.

To check whether a function $f$ is of exponential order, we can show that $\frac{f(t)}{e^{at}}$ is bounded for sufficiently large t.
![[12-2-exp-order-f.png]]

# Properties of the Laplace Transform (5.2)

Suppose $F(s) = \mathcal L\{f(t)\}.$

## Theorems

### Translating Along $s$-domain

$$\mathcal L\{e^{ct}f(t)\} = F(s - c)$$

> [!Info]+ Derivation
> $$
> \begin{align*}
>   \mathcal L\{e^{ct}f\} &= \int_0^\infty fe^{ct}e^{-st}\,dt\\
>   &= \int_0^\infty fe^{-(s-c)t}\,dt\\
>   &= F(s - c)
> \end{align*}
> $$

### Theorem: First Derivative

$$\mathcal L \{f'(t)\} = sF(s) - f(0)$$

> [!Info]+ Derivation
> $$
> \mathcal L\{f'(t)\} = \int_0^\infty f'e^{-st}\,dt
> $$
> 
> Using integration by parts:
> $$
> \begin{align*}\\
> u &= e^{-st} & du &= -se^{-st}dt\\
> dv &= f'dt & v &= f
> \end{align*}
> $$
> 
> Then,
> $$
> \begin{align*}
>   \mathcal L\{f'(t)\} &= \left.\left(e^{-st} f\right)\right|^{t=\infty}_{t=0} - \int_0^\infty\left(-se^{-st}f\right)\,dt\\
>   &= -f(0) + sF(s)
> \end{align*}
> $$

### Theorem: Higher Order Derivatives

$$\mathcal L \{f''(t)\} = s^2F(s) - sf(0) - f'(0)$$
$$\mathcal L \{f^{(n)}(t)\} = s^nF(s) - s^{n-1}f(0) - s^{n-2}f'(0) - \ldots - f^{(n-1)}(0)$$

### Theorem: Derivatives in the $s$-domain
$$
\mathcal L\{t^n f(t)\} = (-1)^n F^{(n)}(s)
$$

> [!Info]+ Derivation
> 
> Note that
> $$
> \begin{align*}
>   \frac{d^nF}{ds^n} &= \frac{d^n}{ds^n} \int_0^\infty e^{-st}f(t)\,dt\\
>   &= (-1)^n\int_0^{\infty}t^n e^{-st}f\,dt\\
>   &= (-1)^n \mathcal L\{t^n f\}
> \end{align*}
> $$
> 
> Using integration by parts:
> $$
> \begin{align*}\\
> u &= e^{-st} & du &= -se^{-st}dt\\
> dv &= f'dt & v &= f
> \end{align*}
> $$
> 
> Then,
> $$
> \begin{align*}
>   \mathcal L\{f'(t)\} &= \left.\left(e^{-st} f\right)\right|^{t=\infty}_{t=0} - \int_0^\infty\left(-se^{-st}f\right)\,dt\\
>   &= -f(0) + sF(s)
> \end{align*}
> $$

It follows from this theorem that
$$
\mathcal L \{t^n\} = \frac{n!}{s^{n+1}}.
$$

## Computing Laplace Transforms of IVPs

> [!Info]+ Motivating Example: First Order DE
> Compute the Laplace Transform of:
> $$
> y' = e^{-6t}\sin(t),\quad y(0) = 2
> $$
> 
> On the left-hand side:
> $$\mathcal L\{y'\} = sY - y(0) = sY - 2$$
> 
> On the right-hand side:
> $$\mathcal L\{e^{-6t}\sin t\} = \frac{1}{(s+6)^2 + 1}$$
> 
> Then:
> $$
> \begin{align*}
>   sY - 2 &= \frac{1}{(s+6)^2 + 1}\\
>   Y &= \frac{2}{s} + \frac{\frac{1}{s}}{(s+6)^2 + 1}
> \end{align*}
> $$

> [!Info]+ Motivating Example: Second Order DE
> Compute the Laplace Transform of:
> $$
> y'' + 9y = e^{-t}\sin(4t),\quad y(0) = 0, y'(0) = 1
> $$
> 
> On the left-hand side:
> $$\mathcal L\{y'' + 9y\} = (s^2Y - sy(0) - y'(0)) + 9Y = (s^2 + 9)Y - 1$$
> 
> On the right-hand side:
> $$\mathcal L\{e^{-t}\sin 4t\} = \frac{4}{(s+1)^2 + 16}$$
> 
> Then,
> $$
> (s^2 + 9)Y = 1 + \frac{4}{(s+1)^2 + 16}
> $$

# Inverse Laplace Transform (5.3)

If $f, g$ are piece-wise continuous and of exponential order, and $$\mathcal L\{f\} = \mathcal L\{g\},$$then $f = g$.

We can define $\mathcal L^-1$ to be the **inverse [[12. Laplace Transform#Definition of Laplace Transform (5.1)|Laplace operator]]**, such that
$$
\mathcal L^{-1} \{\mathcal L\{f\}\} = f.
$$

Note that the Inverse Laplace transform is linear.

## Examples

> [!Example]+ Example: $\mathcal L^{-1}\left\{\frac{4}{s^3}\right\}$
> $$\frac{4}{s^3} = 2 \cdot \frac{2!}{s^3} = 2 \mathcal L \{t^2\}.$$
> 
> Therefore, $$\mathcal L^{-1}\left\{\frac{4}{s^3}\right\}= 2t^2.$$

> [!Example]+ Example: $\mathcal L^{-1}\left\{\frac{3}{s^2 + 9}\right\}$
> $$\frac{3}{s^2 + 9} = \mathcal L {\sin 3t}.$$
> 
> Therefore, $$\mathcal L^{-1}\left\{\frac{3}{s^2 + 9}\right\}= \sin 3t.$$

> [!Example]+ Example: $\mathcal L^{-1}\left\{\frac{s - 1}{s^2 - 2s + 5}\right\}$
> $$\frac{s - 1}{s^2 - 2s + 5} = \frac{(s-1)}{(s-1)^2 + 2^2} = \mathcal L \{e^t \cos 2t\}.$$
> 
> Therefore, $$\mathcal L^{-1}\left\{\frac{s - 1}{s^2 - 2s + 5}\right\} = e^t \cos 2t.$$

> [!Example]+ Example: $\mathcal L^{-1}\left\{\frac{5}{(s + 2)^4}\right\} \overset?= t^ne^{kt}$
> $$\frac{5}{(s + 2)^4} = \frac{5}{6} \cdot \frac{3!}{(s+2)^4} = \mathcal L \left\{\frac{5}{6}t^3 e^{-2t}\right\}.$$

> [!Example]+ Example: Distinct Linear Partial Fractions — $\mathcal L^{-1}\left\{\frac{7s-1}{(s+1)(s+2)(s-3)}\right\}$
> $$\frac{7s-1}{(s+1)(s+2)(s-3)} = \frac{A}{s + 1}+ \frac{B}{s+2} + \frac{C}{s-3}.$$
> 
> As such,
> $$
> 7s - 1 = A(s + 2)(s - 3) + B(s + 1)(s - 3) + C(s + 1)(s + 2).
> $$
> 
> By plugging in $s = -1, -2, 3$, we get...
> $$
> \begin{align*}
>   -8 &= A(-1 + 2)(-1 - 3)\\
>   -15 &= B(-2 + 1)(-2 - 3)\\
>   20 &= C(3 + 1)(3 + 2).
> \end{align*}
> $$
> Then, $A = 2, B = -3, C = 1$.
> 
> As such, $$\mathcal L^{-1}\left\{\frac{7s-1}{(s+1)(s+2)(s-3)}\right\} = 2e^{-t} - 3e^{-2t} + e^{3t}.$$

> [!Example]+ Example: Repeated Linear Partial Fractions — $\mathcal L^{-1}\left\{\frac{s^2 + 9s + 2}{(s-1)^2(s+3)}\right\}$
> $$\frac{s^2 + 9s + 2}{(s-1)^2(s+3)} = \frac{A}{s - 1}+ \frac{B}{(s - 1)^2} + \frac{C}{s+3}.$$
> 
> As such,
> $$
> s^2 + 9s + 2 = A(s - 1)(s + 3) + B(s + 3) + C(s - 1)^2.
> $$
> 
> By plugging in $s = -3$, we get...
> $$-16 = C(-4)^2.$$
> Then, $C = -1$.
> 
> By plugging in $s = 1$, we get:
> $$12 = 4B.$$
> Then $B = 3.$
> 
> We then have 
> $$
> \begin{align*}
>   s^2 + 9s + 2 &= A(s - 1)(s + 3) + 3(s + 3) - (s - 1)^2\\
>   s^2 + 9s + 2 &= A(s^2 + 2s - 3) + 3s + 9 - s^2 + 2s - 1\\
>   2s^2 + 4s - 6 &= A(s^2 + 2s - 3).
> \end{align*}
> $$
> Then, $A = 2$.
> 
> As such, $$\mathcal L^{-1}\left\{\frac{s^2 + 9s + 2}{(s-1)^2(s+3)}\right\} = 2e^t + 3te^t - e^{3t}.$$

# Solving IVPs with Laplace Transforms (5.4)

The process for solving IVPs with Laplace transforms is as follows:
1. Compute $\mathcal L$ for IVP.
2. Solve for $Y(s) = \mathcal L\{y\}$.
3. Compute $\mathcal L^{-1}$ of $Y$ fo find $y$.

> [!Example]+
> $$y' + 3y = 13\sin 2t, \quad y(0) = 6.$$
> 
> LHS:
> $$
> \begin{align*}
>   \mathcal L\{y' + 3y\} &= sY - y(0) + 3Y\\
>   &= (s + 3)Y - 6
> \end{align*}
> $$
> 
> RHS:
> $$
> \mathcal L\{13 \sin 2t\} = \frac{13 \cdot 2}{s^2 + 4}.
> $$
> 
> Therefore,
> $$
> \begin{align*}
>   (s + 3)Y &= 6 + \frac{26}{s^2 + 4}\\
>   Y &= \frac{6}{s + 3} + \frac{26}{(s^2+4)(s + 3)}\\
>   &= \frac{6s^2 + 50}{(s^2+4)(s + 3)}
> \end{align*}
> $$
> 
> Then, we can use partial fraction decomposition:
> $$
> \begin{align*}
>    \frac{6s^2 + 50}{(s^2+4)(s + 3)} &= \frac{A}{s+3} + \frac{Bs + C}{(s^2 + 4)}\\
>    6s^2 + 50 &= A(s^2 + 4) + (Bs + C)(s + 3).
> \end{align*}
> $$
> 
> Plugging in $s = -3$:
> $$
> 6(-3)^2 + 50 = A(9 + 4).
> $$
> Then, $A = 8$.
> 
> Plugging in $s = 0$:
> $$
> 50 = 32 + C(3).
> $$
> Then, $C = 6$.
> 
> Then, by expanding, $B = -2$.
> 
> Then,
> $$
> y = 8e^{-3t} - 2 \cos 2t + 3 \sin 2t.
> $$

# Elementary Laplace Formulas

| $f(t)$                                                       | $\mathcal L[f(t)]$                                  | $s$-domain            |
| ------------------------------------------------------------ | --------------------------------------------------- | --------------------- |
| 1                                                            | $\frac{1}{s}$                                       | $s > 0$               |
| $e^{at}$                                                     | $\frac{1}{s-a}$                                     | $s > a$               |
|                                                              |                                                     |                       |
| $t^n,\ n \in \mathbb{Z}^+$                                   | $\frac{n!}{s^{n + 1}}$                              | $s > 0$               |
| $t^p,\ p > -1$                                               | $\frac{\Gamma(p + 1)}{s^{p + 1}}$                   | $s > 0$               |
|                                                              |                                                     |                       |
| $\sin at$                                                    | $\frac{a}{s^2 + a^2}$                               | $s > 0$               |
| $\cos at$                                                    | $\frac{s}{s^2 + a^2}$                               | $s > 0$               |
| $\sinh at$                                                   | $\frac{a}{s^2 - a^2}$                               | $s > \lvert a \lvert$ |
| $\cosh at$                                                   | $\frac{s}{s^2 - a^2}$                               | $s > \lvert a\lvert$  |
|                                                              |                                                     |                       |
| $u_c (t) = \begin{cases}0, & t < c\\1, & t \ge c\end{cases}$ | $\frac{e^{-cs}}{s}$                                 | $s > 0$               |
| $u_c(t)f(t - c)$                                             | $e^{-cs}F(s)$                                       |                       |
| $e^{ct}f(t)$                                                 | $F(s - c)$                                          |                       |
| $\int_0^t f(t - \tau)g(\tau)\, d\tau$                        | $F(s)G(s)$                                          |                       |
| $\delta (t - c) = \begin{cases}0, & t \ne t_0\\1, & t = t_0\end{cases}$                                             | $e^{-cs}$                                           |                       |
| $f^{(n)}(t)$                                                 | $s^nF(s) - s^{n - 1}f(0) - \ldots - f^{(n - 1)}(0)$ |                       |
| $t^nf(t)$                                                    | $(-1)^n f^{(n)}(s)$                                                    |                       |
