**Textbook sections**: 5.4

See [[12a. Laplace Transform#Definition of Laplace Transform (5.1)|Laplace transforms]] and [[12a. Laplace Transform#Inverse Laplace Transform (5.3)|inverse Laplace transforms]].

# The Process

1. Compute $\mathcal L$ for IVP.
2. Solve for $Y(s) = \mathcal L[y]$.
3. Compute $\mathcal L^{-1}$ of $Y$ fo find $y$.

## Examples

> [!Example]+
> $$y' + 3y = 13\sin 2t, \quad y(0) = 6.$$
> 
> LHS:
> $$
> \begin{align*}
>   \mathcal L[y' + 3y] &= sY - y(0) + 3Y\\
>   &= (s + 3)Y - 6
> \end{align*}
> $$
> 
> RHS:
> $$
> \mathcal L[13 \sin 2t] = \frac{13 \cdot 2}{s^2 + 4}.
> $$
> 
> Therefore,
> $$
> \begin{align*}
>   (s + 3)Y &= 6 + \frac{26}{s^2 + 4}\\
>   Y &= \frac{6}{s + 3} + \frac{26}{(s^2+4)(s + 3)}\\
>   &= \frac{6s^2 + 50}{(s^2+4)(s + 3)}
> \end{align*}
> $$
> 
> Then, we can use partial fraction decomposition:
> $$
> \begin{align*}
>    \frac{6s^2 + 50}{(s^2+4)(s + 3)} &= \frac{A}{s+3} + \frac{Bs + C}{(s^2 + 4)}\\
>    6s^2 + 50 &= A(s^2 + 4) + (Bs + C)(s + 3).
> \end{align*}
> $$
> 
> Plugging in $s = -3$:
> $$
> 6(-3)^2 + 50 = A(9 + 4).
> $$
> Then, $A = 8$.
> 
> Plugging in $s = 0$:
> $$
> 50 = 32 + C(3).
> $$
> Then, $C = 6$.
> 
> Then, by expanding, $B = -2$.
> 
> Then,
> $$
> y = 8e^{-3t} - 2 \cos 2t + 3 \sin 2t.
> $$
