**Textbook sections**: 5.5

> [!Info]+ Motivating Example
> Suppose that at time $t = 0$, we place a pie into an oven whose temperature, $y(t)$, is 20° C.
> - When $t = 0$, the pie and oven are both 20° C.
> - $y(t)$ increases linearly at rate 50°C/min until $t = 4$.
> - For $t \ge 4\text{ min}, y = 220$.
> 
> Construct an IVP that represents this situation. How can we solve it?
> 
> ### Construction
> Let $\Pi(t)$ be the temperature of the pie. Then, from [[01a. Mathematical Models & Solutions#Differential Equations|Newton's Law of Cooling]],
> $$
> \Pi' = -k(\Pi - y).
> $$
> However, $y$ is not constant, and is defined as:
> $$
> y = \begin{cases}20 + 50t,&0 \leq t < 4\\220,& t\geq 4\end{cases}
> $$

# Step and Indicator Functions

The **unit step function** is defined as:
$$
u_c(t) = \begin{cases} 
0, &0 \leq t < c \\
1, & c \leq t
\end{cases}
$$
(The unit step function starts at 0, and increments to 1 at $t = c$.)

The **indicator function** is defined as:
$$
u_{bc}(t) = u_b(t) - u_c(t) = \begin{cases} 
0, &0 \leq t < b \\
1, & b \leq t < c \\
0, &c \le t
\end{cases}
$$
(The indicator function starts at 0, increments to 1 at $t = b$, and drops to 0 at $t = c$.)

## Converting Piecewise Functions

> [!Example]+
> Express the following function in terms of step functions.
> $$
> f(t) = \begin{cases} 
>   2, &0 \leq t < 3 \\
>   -2, & 3 \leq t
> \end{cases}
> $$
> 
> In step functions,
> $$
> \begin{align*}
>   f(t) &= 2u_{03} - 2u_{3}\\
>   &= 2(u_0 - u_3) - 2u_3\\
>   &= 2u_0 - 4u_3.
> \end{align*}
> $$

> [!Example]+
> Express the following function in terms of step functions.
> $$
> g(t) = \begin{cases} 
>   t, &0 \leq t < 2 \\
>   t^2, & 2 \leq t < 4 \\
>   t^3, & 4 \leq t
> \end{cases}
> $$
> 
> In step functions, this can be written as
> $$
> \begin{align*}
>   g(t) &= tu_{02} + t^2u_{24} + t^3u_4\\
>   &= tu_0 - tu_2 + t^2u_2 - t^2u_4 + t^3u_4\\
>   &= tu_0 + (t^2 - t)u_2 + (t^3 - t^2)u_4.
> \end{align*}
> $$

## Laplace of Step Function
$$
\mathcal L \{u_c(t)\} = \frac{e^{-cs}}{s}.
$$
> [!Info]+ Derivation
> $$
> \begin{align*}
>   \mathcal L \{ u_c(t) \} &= \int_c^\infty e^{-st}\,dt\\
>   &= \left.-\frac{1}{s}e^{-st}\right|_{t = c}^{t = \infty}\\
>   &= \frac{1}{s}e^{-sc}
> \end{align*}
> $$

> [!Example]
> Solve the IVP:
> $$y' + y = f,\quad y(0) = 0,\quad f = \begin{cases}1,&0\leq t<1\\-1,&1\leq t\end{cases}$$
> 
> Note that $$\begin{align*}
>   f &= u_{01} - u_1 \\
>   &= (u_0 - u_1) - u_1 \\
>   &= u_0 - 2u_1.
> \end{align*}$$
> 
> Then,
> $$
> \begin{align*}
>   \mathcal L\{ y' + y \} &= sY + y(0) + Y\\
>   &= (s + 1)Y.\\
>   \mathcal L\{f\} &= \frac{1}{s} - \frac{2e^{-s}}{s}.
> \end{align*}$$
> 
> Setting them equal, we find
> $$
> Y = \frac{1}{s(s + 1)} - \frac{2e^{-s}}{s(s + 1)}.
> $$
> 
> Note that $$\frac{1}{s(s + 1)} = \frac{1}{s} - \frac{1}{s + 1}.$$
> 
> Then,
> $$
> \begin{align*}
>   Y &= \frac{1}{s} - \frac{1}{s + 1} - 2e^{-s}\left(\frac{1}{s} - \frac{1}{s + 1}\right) \\
>   &= \frac{1}{s} - \frac{1}{s + 1} - 2\left(\frac{e^{-s}}{s} - \frac{e\cdot e^{-s - 1}}{s + 1}\right) \\
>   &= \mathcal L \{1 - e^{-t} - 2u_1(t) + 2e^{-t}u_1(t)\}.
> \end{align*}
> $$
> 
> Therefore,
> $$y = 1 - e^{-t} - 2u_1(t) + 2ee^{-t}u_1(t).$$

### Shift in $t$-Domain
$$
\mathcal L \{u_c(t) f(t-c)\} = e^{-cs}F(s)
$$
> [!Info]+ Derivation
> $$
> \begin{align*}
>   \mathcal L \{ u_c(t) f(t-c) \} &= \int_c^\infty f(t - c) e^{-st}\,dt.
> \end{align*}
> $$
> 
> Let $G = t - c, dG = dt$.
> When $t \to c,\ G \to 0$, and when $t \to \infty,\ G \to \infty.$
> Then,
> $$
> \begin{align*}
>   \mathcal L \{ u_c(t) f(t-c) \} &= \int_0^\infty f(G)e^{-s(G + c)}\,dG\\
>   &= e^{-sc}\mathcal L\{f\}.
> \end{align*}
> $$

> [!Example]+
> Compute $$\mathcal L^{-1}\left\{\frac{1}{s - 4}e^{-2s}\right\}.$$
> 
> Note that $c = 2$ and $\mathcal L\{e^{4t}\} = \frac{1}{{s-4}}$. Then,
> $$
> \begin{align*}
>    \mathcal L^{-1}\left\{\frac{1}{s - 4}e^{-2s}\right\} &= u_{2}e^{4(t - 2)}.
> \end{align*}
> $$

# Periodic Functions

Suppose $f(t)$ is a periodic function with period $T$. Then,
$$
\mathcal L\{f(t)\} = \frac{1}{1-e^{-Ts}}\int_0^T e^{-st}f(t)\,dt
$$

> [!Info]+ Derivation
> $$
> \begin{align*}
>   \mathcal L\{f\} &= \int_0^\infty e^{-st}f\,dt\\
>   &= \int_0^T e^{-st}f\,dt + \int_T^\infty e^{-st}f\,dt.
> \end{align*}
> $$
> 
> Let $u = t - T,\ du = dt$.
> When $t \to T,\ u\to0,$ and when $t\to\infty,\ u\to\infty$. Then,
> $$
> \begin{align*}
>   \mathcal L\{f\} &= \int_0^T e^{-st}f\,dt + \int_0^\infty e^{-s(u + T)}\overbrace{f(u + T)}^{f(u)}\,du\\
>   &= \int_0^T e^{-st}f\,dt + e^{-Ts}\int_0^\infty e^{-su}f\,du.
> \end{align*}
> $$
> Then,
> $$
> \begin{align*}
>   \int_0^\infty e^{-st}f\,dt &= \int_0^T e^{-st}f\,dt + e^{-Ts}\int_0^\infty e^{-su}f\,du\\
>   (1 - e^{-Ts})\int_0^\infty e^{-st}f\,dt &= \int_0^T e^{-st}f\,dt\\
>   \int_0^\infty e^{-st}f\,dt &= \frac{1}{1 - e^{-Ts}}\int_0^T e^{-st}f\,dt.
> \end{align*}
> $$

## Examples

![[13a-1-periodic-example.png]]
> [!Example]+ Example: $y_1$
> 
> This function repeats every $2a$. As such,
> $$
> \begin{align*}
>   \mathcal L\{y_1\} &= \frac{1}{1-e^{-2as}}\int_0^{2a} e^{-st}f(t)\,dt\\
>   &= \frac{1}{1-e^{-2as}}\left(\int_0^a e^{-st}\,dt - \int_a^{2a} e^{-st}\,dt\right)\\
>   &= \frac{1}{1-e^{-2as}}\left(- \frac{1}{s}(e^{-as} - 1) + \frac{1}{s}(e^{-2as}-e^{-as})\right)
> \end{align*}
> $$
