**Textbook sections**: 5.8

> [!Info]+ Motivating Example
> Consider the spring-mass system
> $$y'' + \omega^2 y = g(t),\quad y(0)=0,\quad y'(0) = 0,$$
> such that $w^2 = \frac{k}{m}.$
> 
> If $g(t)$ is unknown, can we express $y(t)$ in terms of $g(t)$? How?
> 
> 1. Variation of Parameters
> 2. Convolutions and $\mathcal L$
>    
> ### Using Convolutions & $\mathcal L$
> Take $\mathcal L$ of both sides of our DE: 
> $$
> \begin{align*}
>   \mathcal L\{y'' + \omega^2 y\} &= \mathcal L\{g\}\\
>   s^2 Y - sy(0) - y'(0) + \omega^2 Y &= G\\
>   (s^2 + \omega^2)Y &= G\\
>   Y &= \frac{1}{s^2 + \omega^2}G\\
>   &= \frac{1}{\omega}\frac{\omega}{s^2 + \omega^2}G.
> \end{align*}
> $$
> This could be computed if we had a way to compute $$\mathcal L^{-1}\{F(s)G(s)\}$$ for arbitrary $F$ and $G$.

# Convolutions

The **convolution** between piecewise continuous functions $f$ and $g$ is
$$
f * g = \int_0^t f(t - \tau)g(\tau)\,d\tau.
$$

Some useful properties:

| property     | identity                              |
| ------------ | ------------------------------------- |
| commutative  | $f * g = g * f$                       |
| distributive | $f * (g_1 + g_2) = f * g_1 + f * g_2$ |
| associative  | $(f * g) * h = f * (g * h)$           |
| zero         | $f * 0 = 0 * f = 0$                   |

## Convolution Theorem

Let $f$ and $g$ be functions such that $\mathcal L\{f\} = F$ and $\mathcal L\{g\} = G$. Then:
$$
\mathcal L\{f * g\} = F(s)G(s).
$$

> [!Info]+ Derivation
> 
> Note that
> $$
> \begin{align*}
>   F(s) &= \int_0^\infty e^{-s\xi}f(\xi)\,d\xi\\
>   G(s) &= \int_0^\infty e^{-s\tau}g(\tau)\,d\tau.
> \end{align*}
> $$
> 
> Then,
> $$
> F(s)G(s) = \int_0^\infty e^{-s\xi}f(\xi)\,d\xi\int_0^\infty e^{-s\tau}g(\tau)\,d\tau.
> $$
> 
> Since these integrals are not dependent on each other, we can merge them into a double integral:
> $$
> \begin{align*}
>   F(s)G(s) &= \int_0^\infty e^{-s\tau}g(\tau)\left(\int_0^\infty e^{-s\xi}f(\xi)\,d\xi\right)\,d\tau\\
>   &= \int_0^\infty g(\tau)\left(\int_0^\infty e^{-s(\xi + \tau)}f(\xi)\,d\xi\right)\,d\tau.
> \end{align*}
> $$
> 
> Let $t = \xi + \tau$ for select $\tau$. Then, $dt = d\xi$. 
> When $\xi \to 0,\ t \to \tau,$ and when $\xi \to \infty,\ t \to \infty.$
> 
> $$
> \begin{align*}
>   F(s)G(s) &= \int_0^\infty g(\tau)\left(\int_\tau^\infty e^{-st}f(t - \tau)\,dt\right)\,d\tau.
> \end{align*}
> $$
> 
> We can use change of variable to find that
> $$
> \int_0^\infty \int_\tau^\infty (\ldots) \,dt\,d\tau \to \int_0^\infty \int_0^t (\ldots) \,d\tau\,dt.
> $$
> 
> Hence,
> $$
> \begin{align*}
>   F(s)G(s) &= \int_0^\infty e^{-st} \left(\int_\tau^\infty f(t - \tau)g(\tau)\,d\tau\right)\,dt\\
>   &= \mathcal L\{f * g\}.
> \end{align*}
> $$

> [!Example]+ Continuing the Motivating Example
> $$Y = \frac{1}{\omega}\frac{\omega}{s^2 + \omega^2}G.$$
> 
> Using the Convolution Theorem, we see that
> $$
> \begin{align*}
>   Y &= \frac{1}{\omega}\mathcal L\{\sin \omega t\}\cdot \mathcal L\{g(t)\}\\
>   &= \frac{1}{\omega}\mathcal L\{\sin \omega t * g(t)\}.
> \end{align*}
> $$
> 
> Therefore,
> $$
> y = \frac{1}{\omega}\int_0^t \sin(\omega (t - \tau))g(\tau)\,d\tau.
> $$

> [!Example]+
> Compute the inverse Laplace Transform of the function:
> $$
> \frac{1}{(s^2 + 1)^2}
> $$
> 
> We see that
> $$
> \begin{align*}
>   \frac{1}{(s + 1)^2} &= \frac{1}{s^2 + 1} \cdot \frac{1}{s^2 + 1}\\
>   &= \mathcal L\{\sin t\}\cdot\mathcal L\{\sin t\}\\
>   &= \mathcal L\{\sin t * \sin t \}.
> \end{align*}
> $$
> 
> Hence, $$
> \begin{align*}
>   \mathcal L^{-1}\left\{\frac{1}{(s + 1)^2}\right\} &= \sin t * \sin t\\
>   &= \int_0^t \sin(t-\tau)\sin\tau\,d\tau
> \end{align*}
> $$

> [!Example]+
> Compute the inverse Laplace Transform of the function:
> $$
> \frac{14}{(s + 2)(s - 6)}
> $$
> 
> $$
> \begin{align*}
>   \mathcal L\left\{\frac{14}{(s + 2)(s - 6)}\right\} &= 14 \int_0^t e^{-2(t-\tau)}e^{6\tau}\,d\tau\\
>   &= 14 e^{-2t}\int_0^t e^{8\tau}\,d\tau\\
>   &= 14 e^{-2t} \cdot \frac{1}{8}(e^{8t} - 1)
> \end{align*}
> $$

