# Complex Eigenvalues
Given a complex eigenvalue and eigenvector:
$$
\begin{matrix}
\lambda_1 = \alpha_1 + i\beta_1 & \vec v_1 = \vec a_1 + i\vec b_1\\
%%\lambda_2 = \alpha_2 + i\beta_2 & \vec v_2 = \vec a_2 + i\vec b_2%%
\end{matrix}
$$

Then, we see that a solution is:
$$
\begin{align*}
\vec u &= e^{\lambda t}\vec v\\
&= e^{\alpha t}e^{i \beta t}(\vec a + i \vec b)\\
&= e^{\alpha t}(\cos (\beta t) + i\sin(\beta t))(\vec a + i \vec b)\\
&= e^{\alpha t}((\vec a\cos (\beta t) - \vec b \sin (\beta t)) + i(\vec a \sin (\beta t) + \vec b \cos (\beta t)))\\
&= \overbrace{e^{\alpha t}(\vec a \cos (\beta t) - \vec b\sin (\beta t) )}^{\vec x_1} + i\overbrace{ e^{\alpha t}(\vec a\sin (\beta t) + \vec b \cos (\beta t))}^{\vec x_2}\\
&= \vec x_1 + i\vec x_2
\end{align*}
$$

Hence, the general solution is
$$
\begin{align*}
\vec x_1 &= e^{\alpha t}(\vec a \cos (\beta t) - \vec b\sin (\beta t) )\\
\vec x_2 &= e^{\alpha t}(\vec a\sin (\beta t) + \vec b \cos (\beta t))\\
\vec x &= c_1 \vec x_1 + c_2 \vec x_2
\end{align*}
$$
*Note that the conjugate eigenvalue and eigenvector will result in the same $\vec x_1$ and $\vec x_2$.*

## Example
Determine general solution to
$$
\vec x' = \begin{bmatrix}-1 & 2 \\ -1 & -3\end{bmatrix}\vec x
$$
### Computing eigenthings
Eigenvectors:
$$
\begin{align*}
(-1-\lambda)(-3-\lambda)+2 &= 0\\
\lambda^2 +4\lambda+5&=0\\
\lambda&=-2\pm \sqrt{4 - 5}\\
&= -2 \pm i
\end{align*}
$$
Eigenvalues:
$$(A - \lambda I)\vec v = \begin{bmatrix}-1-\lambda & 2 \\ -1 & -3 - \lambda\end{bmatrix} \vec v = 0$$
$\lambda_1 = - 2 - i$:
$$A - \lambda I = \begin{bmatrix}1 + i & 2 \\ -1 & -1 + i\end{bmatrix}$$
$$\vec v_1 = \begin{bmatrix}-1 + i \\ 1\end{bmatrix}$$
$\lambda_2 = - 2 + i$:
$$A - \lambda I = \begin{bmatrix}1 - i & 2 \\ -1 & -1 - i\end{bmatrix}$$
$$\vec v_2 = \begin{bmatrix}-1 - i \\ 1\end{bmatrix}$$
### General solution

Using $\lambda_2 = -2 + i$:
$$\begin{align*}
\alpha &= -2,\\
\beta &= 1\\
\vec a &= \begin{bmatrix}-1 \\ 1\end{bmatrix}\\
\vec b &= \begin{bmatrix}-1 \\ 0\end{bmatrix}
\end{align*}$$

So the general solution:
$$
\begin{align*}
\vec x_1 &= e^{-2t}\left(\begin{bmatrix}-1 \\ 1\end{bmatrix}\cos t - \begin{bmatrix}-1 \\ 0\end{bmatrix} \sin t\right)\\
\vec x_2 &= e^{-2t}\left(\begin{bmatrix}-1 \\ 1\end{bmatrix}\sin t + \begin{bmatrix}-1 \\ 0\end{bmatrix} \cos t\right)\\
\vec x &= c_1 \vec x_1 + c_2 \vec x_2
\end{align*}
$$

## Phase Portraits
It either moves toward or away from the origin, if $\alpha$ is negative or positive.
It will do a spiral (rotation-esque) motion:
![[Pasted image 20230114115032.png]]

To determine if that spiral is clockwise or counterclockwise, test a point (e.g. $\begin{bmatrix}1 \\ 0\end{bmatrix}$ and $\begin{bmatrix}0 \\ 1\end{bmatrix}$) and see where the rotation points.

Given $\lambda = \alpha + i \beta$:
|Eigenvalues|Sample phase portrait|Type of critial point|stability|
|-|-|-|-|
|$\alpha < 0$|![[Pasted image 20230114115454.png]]|(0, 0) is a *spiral sink*|asymptotically stable|
|$\alpha > 0$|![[Pasted image 20230114115541.png]]|(0, 0) is a *spiral source*|unstable|
|a = 0|![[Pasted image 20230114115606.png]]|(0, 0) is a *center*|stable|

# Repeated Eigenvalues

In a situation where there's a repeated eigenvalue but not two eigenvectors, the solution found will be:
$$
\vec r(t) = c_1 e^{\lambda t} \vec v + c_2 e^{\lambda t}(\vec vt + \vec w)
$$

$w$ can be found by $(A - \lambda I)\vec w = \vec v$.

## Example 1
Given an object moving in the plane with motion $\vec{r}(t) = \begin{bmatrix}x(t) \\ y(t)\end{bmatrix}$,
such that the velocity is defined as:
$$
\begin{align*}
x' &= -x + ky\\
y' &= -y
\end{align*}
$$
and such that $\vec{r}(0) = \begin{bmatrix}1 \\ 2\end{bmatrix}$.

### If $k = 0$

#### Solving
$$\begin{align*}
\frac{d\vec r}{dt} = \begin{bmatrix}-1 & 0 \\ 0 & -1\end{bmatrix}\vec r
\end{align*}$$
##### Eigenvalues
$$(-1 - \lambda)^2 = 0$$
So $\lambda_1 = \lambda_2 = -1$.

The eigenvectors are: $\left\{\begin{bmatrix}1 \\ 0\end{bmatrix}, \begin{bmatrix}0 \\ 1\end{bmatrix}\right\}$

#### Phase Portrait
![[Pasted image 20230114120544.png]]

### If $k \neq 0$

#### Solving
There aren't two eigenvectors so we can't use the matrix method.

Given
$$
\begin{align*}
x' &= -x + ky\\
y' &= -y,
\end{align*}
$$
$y = c_2e^{-t}$.

Then, we can solve for $x' + x = ky$:
$$
\begin{align*}
e^{t}x' + e^tx &= e^t ky\\
e^t x &= \int kc_2\,dt\\
x &= \frac{kc_2t}{e^t} + \frac{c_1}{e^t}
\end{align*}
$$

Hence:
$$
\begin{align*}
\vec{r} &= \begin{bmatrix}c_1e^{-t} + kc_2te^{-t} \\ c_2e^{-t} \end{bmatrix}\\
&= c_1e^{-t}\begin{bmatrix}1 \\ 0\end{bmatrix} + c_2e^{-t}\left(\begin{bmatrix}1 \\ 0\end{bmatrix}kt + \begin{bmatrix}0 \\ 1\end{bmatrix}\right)
\end{align*}
$$
$\begin{bmatrix}1 \\ 0\end{bmatrix}$ is an eigenvector here, and the phase portrait will move towards the origin along $\left(\begin{bmatrix}1 \\ 0\end{bmatrix}kt + \begin{bmatrix}0 \\ 1\end{bmatrix}\right)$.

#### Phase Portrait
![[Pasted image 20230114122059.png]]

## Example 2
$$\vec x' = \begin{bmatrix}1 & -1 \\ 1 & 3\end{bmatrix}\vec{x}$$

$\lambda_1 = \lambda_2 = 2$, $\vec v = \begin{bmatrix}1 \\ -1\end{bmatrix}$.

Hence, $\vec x_1 = e^{2t}\begin{bmatrix}1 \\ -1\end{bmatrix}$.

## Finding $\vec w$

Is there another linearly independent solution?

Assume $$\vec x_2 = te^{2t}\vec v + e^{2t}\vec w.$$
Note that:
$$
\begin{align*}
\vec x_2' &= \frac{d}{dt}(te^{2t}\vec v + e^{2t}\vec w)\\
&= e^{2t}\vec v + 2te^{2t}\vec v + 2e^{2t}\vec{w},
\end{align*}
$$
and:
$$
\begin{align*}
\vec{x}_2' &= \begin{bmatrix}1 & -1 \\ 1 & 3\end{bmatrix}\vec{x}_2\\
&= A(te^{2t}\vec v + e^{2t}\vec w).
\end{align*}
$$

Setting these equal, we have
$$
\begin{align*}
e^{2t}\vec v + 2te^{2t}\vec v + 2e^{2t}\vec{w} &= A(te^{2t}\vec v + e^{2t}\vec w)\\
\vec v + 2t\vec v + 2\vec{w} &= A(t\vec v) + A\vec w
\end{align*}
$$

Aligning the $t$ and non-$t$ terms:
$$
\begin{align*}
A(t\vec{v}) &= 2t\vec v\\
\vec v + 2\vec w &= A\vec w
\end{align*}
$$
We are trying to find $(A - 2I)\vec w = \vec v$, so solve:
$$
\begin{bmatrix}
-1 & -1 \\ 1 & 1
\end{bmatrix} \vec w = \begin{bmatrix}-1 \\-1\end{bmatrix}
$$

So, $\vec w = \begin{bmatrix}1 \\ 0\end{bmatrix}$.

